
# (x-y^3)^4

```

4           4             4                 4                   4
  x^4 (1)     x^3(-y)^3     x^2(-y^3)^3       x^1(-y^3)^3         (1)(-y^3)^4
0           1             2                 3                   4

4C0 = 1     4C1 = 4       4C2 = 6           4C3 = 4             4C4 = 1

x^4     -   4x^3y^3   +   6x^2y^6     -     4xy^9         +     y^12

```

# (2x-y^2)^3
```

3               3                 3                 3                   
  (2x)^3 (1)     (2x)^2(-y^2)^1    (2x)^1(-y^2)^2    (1)(-y^2)^3   
0               1                 2                 3

3C0 = 1         3C1 = 3           3C2 = 3           3C3 = 1

8x^3     -   12x^2y^2   +   6xy^4     -     y^6

```
